update before I start from scratch

transitive_closure.v
@@ -1,7 +1,857 @@
-Require Import ssreflect ssrbool ssrnat fintype eqtype seq ssrfun.
+Require Import ssreflect ssrbool ssrnat fintype eqtype seq ssrfun ssrbool.
 Require Import automata misc regexp.
 
+Set Implicit Arguments.
+
 (* http://krchowdhary.com/toc/dfa-to-reg-exp.pdf *)
+
+
+
+Section TransitiveClosure.
+
+Variable char: finType.
+Variable A: nfa char.
+
+
+
+Lemma mem_der_Plus r s w : mem_der (@Plus char r s) w = mem_der r w || mem_der s w.
+Proof. elim: w r s => [|a w IHw] r s //=. Qed.
+
+Lemma der_Plus a r s : der a (@Plus char r s) = Plus (der a r) (der a s).
+Proof. by []. Qed.
+
+Lemma mem_der_Conc r s (w1 w2: word char) : mem_der r w1 ->  mem_der s w2 ->
+mem_der (Conc r s) (w1 ++ w2).
+Proof.
+elim: w1 r s w2 => [|a w1 IHw1] r s w2 B C /=.
+  elim: w2 r s B C => [|b w2 IHw2] /= r s -> //. 
+  move => C. rewrite mem_der_Plus.
+  by rewrite C orbT.
+case: (has_eps r) => /=.
+  rewrite mem_der_Plus. by rewrite IHw1 => //.
+by apply/IHw1 => //.
+Qed.
+
+
+Lemma der_fold_Plus (r: regular_expression char) rs (a: char): der a (foldr (@Plus char) r rs) = foldr (@Plus char) (der a r) (map (der a) rs).
+Proof.
+elim: rs r a => [|s rs IHrs] r a //=.
+by rewrite IHrs.
+Qed.
+
+Lemma mem_der_fold_Plus r rs w: mem_der r w || has (fun r => mem_der r w) rs = mem_der (foldr (@Plus char) r rs) w.
+Proof.
+  elim: rs r w => [|s rs IHrs] r w.
+    apply/orP/idP.
+      move => [] //=.
+    by firstorder.
+  rewrite /= mem_der_Plus.
+  apply/orP/idP.
+    move => [] H0; apply/orP.
+      right. rewrite -IHrs. by rewrite H0.
+    apply/orP. move/orP: H0 => [].
+      by move => ->.
+    rewrite -IHrs => ->.
+    apply/or3P. by firstorder.
+  move/orP => [].
+    move => ->. by firstorder.
+  rewrite -IHrs. move/orP => [].
+    by firstorder.
+  move => ->. right. by rewrite orbT.
+Qed.
+  
+Lemma has_eps_fold_Plus r rs: has_eps r || has (@has_eps _) rs = has_eps (foldr (@Plus char) r rs).
+Proof.
+  elim: rs r => [|s rs IHrs] r.
+    by rewrite orbF.
+  simpl. rewrite -(IHrs r).
+  by rewrite orbCA.
+Qed.
+
+Lemma mem_der_Void w: mem_der (@Void char) w = false.
+Proof. elim: w => [|a w IHw] //=. Qed.
+
+Lemma mem_der_Eps w: mem_der (@Eps char) w -> w = [::].
+Proof. elim: w => [|a w IHw] //=. by rewrite mem_der_Void. Qed.
+
+Lemma mem_der_Atom a w: mem_der (@Atom char a) w -> w = [::a].
+Proof. elim: w a => [|b w IHw] a //=. case_eq (b==a).
+  by move/eqP => -> /mem_der_Eps ->.
+by rewrite mem_der_Void.
+Qed.
+
+Lemma cons_eq a b (w1 w2: word char):
+  a::w1 = b::w2 -> a=b /\ w1 = w2.
+Proof.
+  move => H0.
+  move: (f_equal (head a) H0) => /=.
+  by move: (f_equal behead H0) => /=.                                   
+Qed.
+                                    
+Lemma mem_der_Conc3 r s w:
+(exists w1, exists w2, w1 ++ w2 = w /\ mem_der r w1 /\ mem_der s w2) -> mem_der (@Conc char r s) w.
+Proof.
+  elim: w r s => [|a w IHw] r s /=.
+    move => [] w1 [] w2 [].
+    case: w1 => [] //. case: w2 => [] //=.
+    by move => _ [] -> ->.
+  move => [] w1 [] w2 [].
+  case_eq (has_eps r) => H0.
+    rewrite mem_der_Plus.
+    case: w1 => [|b w1].
+      move => /= -> [] _ /= ->.
+      by rewrite orbT.
+    rewrite cat_cons.
+    move/cons_eq => [] -> <- [] H1 H2.
+    by rewrite mem_der_Conc.
+  case: w1 => [|b w1].
+    move => _ [] /=. by rewrite H0. 
+  rewrite cat_cons.
+  move/cons_eq => [] -> <- [] H1 H2.
+  by rewrite mem_der_Conc.  
+Qed.
+
+
+Lemma mem_der_Conc2 r s w: mem_der (@Conc char r s) w -> exists w1, exists w2, w1 ++ w2 = w /\ mem_der r w1 /\ mem_der s w2.
+Proof.
+  elim: w r s => [|a w IHw] r s /=.
+    move => /andP [H0 H1].
+    exists [::]. by exists [::].
+  case_eq (has_eps r) => H0.
+    rewrite mem_der_Plus => /orP [].
+      move/IHw => [] w1 [] w2 [] <- [] H1 H2.
+      exists (a::w1). exists w2.
+      split.
+        by [].
+      by rewrite /= H1 H2.
+    move => H1.
+    exists [::]. exists (a::w).
+    split.
+      by [].
+    by rewrite /= H0 H1.
+  move/IHw => [] w1 [] w2 [] <- [] H1 H2.
+  exists (a::w1). exists w2.
+  split.
+    by [].
+  by rewrite /= H1 H2.
+Qed.
+
+Lemma mem_der_Star r w: mem_der (@Star char r) w -> w = [::] \/ mem_der (Conc r (Star r)) w.
+Proof.
+  elim: w r => [|a w IHw] r /=.
+    by firstorder.
+  move/mem_der_Conc2 => [] w1 [] w2 [] H0 [] H1 H2.
+  right.
+  rewrite -H0.
+  case_eq (has_eps r) => H3.
+    rewrite mem_der_Plus.
+    apply/orP. left.
+    by rewrite mem_der_Conc.
+  by rewrite mem_der_Conc.
+Qed.
+  
+Lemma minn_to_ord m n: minn m n <= n.
+Proof. elim: n m => [|n IHn] m /=.
+  by rewrite /minn.
+rewrite /minn.
+case_eq (m < n.+1).
+  by apply: ltnW.
+move => _. by apply: ltnSn.
+Qed.
+
+Lemma noname n m: m > 0 -> n <= m.-1 -> n < m.
+Proof.  elim: m n => [|m IHm] n //=. Qed.
+
+Lemma A_has_states: #|A| > 0.
+apply/card_gt0P.
+by exists (nfa_s0 A).
+Qed.
+  
+(* this represents k in 'I_#|A| *)
+Definition k1_ord k := 
+  Ordinal (noname _ _ A_has_states (minn_to_ord k #|A|.-1)).
+  
+Fixpoint R (k: nat) (i j: 'I_#|A|) : regular_expression char :=
+match k with
+|   0  => 
+      let r := foldr (@Plus _) (Void _) (map (@Atom _) (filter [pred a | nfa_step A (enum_val i) a (enum_val j)] (enum char))) in
+      if i == j then Plus r (Eps _) else r
+| k.+1 =>
+    let k' := k1_ord k in
+    Plus (
+        Conc (R k i k')
+             (Conc (Star (R k k' k')) (R k k' j))
+        )
+        (R k i j)
+end.        
+
+Definition nfa_R (k: nat) (i j: 'I_#|A|) : nfa char :=
+nfaI
+  char
+  (A)
+  (nfa_s0 A)
+  [pred x | x == enum_val j]
+  (fun x a y => nfa_step A x a y && ((enum_rank x == i) || (enum_rank x < k)) && ((enum_rank y == j) || (enum_rank y < k))).
+
+Lemma nfa_R_correct2_0 w i j: mem_der (R 0 i j) w -> nfa_accept (nfa_R 0 i j) (enum_val i) w.
+Proof.
+  elim: w i j => [|a w IHw] i j.
+    simpl.
+    case_eq (i==j).
+      by move/eqP => ->.
+    move => H0. rewrite H0.
+    rewrite -has_eps_fold_Plus. 
+    rewrite orFb.
+    move/hasP => [] r.
+    by move/mapP => [] a _ ->.
+  case_eq (i==j) => /=.
+    move/eqP => ->. rewrite eq_refl /=.
+    rewrite der_fold_Plus mem_der_Plus.
+    rewrite -mem_der_fold_Plus.
+    rewrite mem_der_Void.
+    rewrite orbF orFb.
+    move/hasP => [] r /mapP [] s /mapP [] c.
+    rewrite mem_filter /= => /andP [] H0 _.
+    move => -> -> /=.
+    case_eq (a==c) => /=.
+      move/eqP => ->.
+      move/mem_der_Eps => H1.
+      rewrite H1. rewrite H1 in IHw.
+      apply/existsP. exists (enum_val j).
+      by rewrite enum_valK eq_refl H0 /= eq_refl.
+    by rewrite mem_der_Void.  
+  move => H0. rewrite H0.  
+  rewrite der_fold_Plus -mem_der_fold_Plus mem_der_Void orFb.
+  move/hasP => [] r /mapP [] s /mapP [] c.
+  rewrite mem_filter => /= /andP [] H1 _.
+  move => -> -> /=.
+  case_eq (a==c) => /=.
+    move/eqP => ->. move/mem_der_Eps => ->.
+    apply/existsP. exists (enum_val j).
+    by rewrite 2!enum_valK 2!eq_refl /= H1 eq_refl.
+  by rewrite mem_der_Void.  
+Qed.
+
+Lemma nfa_R_monotone k w i j x: nfa_accept (nfa_R k i j) x w -> nfa_accept(nfa_R k.+1 i j) x w.
+Proof.
+  elim: w k i j x => [|a w IHw] k i j x //=.
+  move/pred0Pn.
+  move => [] y /andP [] /andP [] /andP [] H0 /orP [] H1 /orP [] H2 H3;
+  apply/pred0Pn; exists y.
+        rewrite H0 H1 H2 /=.
+        by apply: IHw.
+      rewrite H0 H1 (leqW H2) orbT /=.
+      by apply: IHw.
+    rewrite H0 (leqW H1) H2 orbT /=.
+    by apply: IHw.
+  rewrite H0 (leqW H1) (leqW H2) 2!orbT /=.
+  by apply: IHw.
+Qed.
+
+Lemma enum_rank_ltn (x: A): enum_rank x <= #|A|.-1.
+Proof.
+  rewrite -(leq_add2r 1) 2!addn1.
+  rewrite (prednK A_has_states).
+  exact: (ltn_ord (enum_rank x)) => /=.
+Qed.  
+
+Lemma k1_ord_leq_k k: nat_of_ord (k1_ord k) <= k.
+Proof.
+  rewrite /k1_ord.
+  case_eq (k <= #|A|.-1) => H0 /=.
+    by rewrite (minnl H0).
+  move: (leq_total k #|A|.-1).
+  rewrite H0 orFb => H1.
+  by rewrite (minnr H1).
+Qed.
+  
+Lemma nfa_R_lpath_start k i j x xs a w:
+  nfa_lpath (nfa_R k i j) x xs (a::w) ->
+  (enum_rank x == i) || (enum_rank x < k).
+Proof.
+  elim: xs => [|y xs IHxs] //.
+  by move => /= /andP [] /andP [] /andP [].
+Qed.          
+
+Lemma nfa_R_lpath_empty k i j x xs:
+  nfa_lpath (nfa_R k i (k1_ord k)) x xs [::] ->
+  nfa_lpath (nfa_R k i j) x xs [::].
+Proof.
+  elim: xs x => [|y xs IHxs] x //=.
+Qed.  
+
+Lemma nfa_R_lpath_empty2 k i j x xs:
+  nfa_lpath (nfa_R k i j) x xs [::] ->
+  nfa_lpath (nfa_R k i (k1_ord k)) x xs [::].
+Proof.
+  elim: xs x => [|y xs IHxs] x //=.
+Qed.  
+
+Lemma nfa_R_correct2' k i j x xs w : 
+  nfa_lpath (nfa_R k i (k1_ord k)) x xs w ->
+  nfa_lpath (nfa_R k.+1 i j) x xs w.
+Proof.
+  elim: w k i j x xs => [|a w IHw] k i j x xs; elim: xs => [|y xs _]  //.
+  move => /= /andP [] /andP [] /andP [] H0 /orP [] H2 /orP [] H3 H4;
+  rewrite H0 2!ltnS.
+        rewrite H2 (eqP H3) (k1_ord_leq_k) orbT /=.
+        by apply: IHw.
+      rewrite H2 (ltnW H3) orbT /=.
+      by apply: IHw.
+    rewrite (ltnW H2).
+    move/eqP: H3 => /(@f_equal 'I_#|A| nat (@nat_of_ord #|A|)) /eq_leq H3.
+    rewrite (leq_trans H3 (k1_ord_leq_k k)) 2!orbT /=.
+    by apply: IHw.
+  rewrite (ltnW H2) (ltnW H3) 2!orbT /=.
+  by apply: IHw.
+Qed.        
+
+Lemma nfa_R_correct2'' k i j x xs w : 
+  nfa_lpath (nfa_R k (k1_ord k) j) x xs w ->
+  nfa_lpath (nfa_R k.+1 i j) x xs w.
+Proof.
+  elim: w k i j x xs => [|a w IHw] k i j x xs; elim: xs => [|y xs _]  //.
+  move => /= /andP [] /andP [] /andP [] H0 /orP [] H2 /orP [] H3 H4;
+  rewrite H0 2!ltnS.
+        move/eqP: H2 => /(@f_equal 'I_#|A| nat (@nat_of_ord #|A|)) /eq_leq H5.
+        rewrite H3 (leq_trans H5 (k1_ord_leq_k k)) orbT /=.
+        by apply: IHw.
+      move/eqP: H2 => /(@f_equal 'I_#|A| nat (@nat_of_ord #|A|)) /eq_leq H5.
+      rewrite (ltnW H3) (leq_trans H5 (k1_ord_leq_k k)) 2!orbT /=.
+      by apply: IHw.
+    rewrite (ltnW H2) H3 orbT /=.
+    by apply: IHw.
+  rewrite (ltnW H2) (ltnW H3) 2!orbT /=.
+  by apply: IHw.
+Qed.
+
+Lemma nfa_R_correct2''' k i j x xs w : 
+  nfa_lpath (nfa_R k (k1_ord k) (k1_ord k)) x xs w ->
+  nfa_lpath (nfa_R k.+1 i j) x xs w.
+Proof.
+  elim: w k i j x xs => [|a w IHw] k i j x xs; elim: xs => [|y xs _]  //.
+  move => /= /andP [] /andP [] /andP [] H0 /orP [] H2 /orP [] H3 H4;
+  rewrite H0 2!ltnS.
+        move/eqP: H2 => /(@f_equal 'I_#|A| nat (@nat_of_ord #|A|)) /eq_leq H5.
+        rewrite (leq_trans H5 (k1_ord_leq_k k)) orbT /=.
+        move/eqP: H3 => /(@f_equal 'I_#|A| nat (@nat_of_ord #|A|)) /eq_leq H6.
+        rewrite (leq_trans H6 (k1_ord_leq_k k)) orbT /=.
+        by apply: IHw.
+      move/eqP: H2 => /(@f_equal 'I_#|A| nat (@nat_of_ord #|A|)) /eq_leq H5.
+      rewrite (ltnW H3) (leq_trans H5 (k1_ord_leq_k k)) 2!orbT /=.
+      by apply: IHw.
+    rewrite (ltnW H2) orbT /=.
+    move/eqP: H3 => /(@f_equal 'I_#|A| nat (@nat_of_ord #|A|)) /eq_leq H6.
+    rewrite (leq_trans H6 (k1_ord_leq_k k)) orbT /=.
+    by apply: IHw.
+  rewrite (ltnW H2) (ltnW H3) 2!orbT /=.
+  by apply: IHw.
+Qed.
+
+(*
+Lemma mem_der_Star_ind (p: word char -> Prop) r:
+  p [::] ->
+  (forall w1 w2, mem_der r w1 -> mem_der (Star r) w2 -> p w2 -> p (w1 ++ w2)) ->
+  forall (w: word char), mem_der (Star r) w -> p w.
+Proof.
+  move => H0 H1 w.
+  move/mem_der_Star => [].
+    by move => ->.
+  move/mem_der_Conc2 => [] w1 [] w2 [] <- [].
+  move => H2 H3.
+  apply: H1 => //.
+          
+    
+  elim: w2 w1 => [|a w2 IHw2] w1.
+    move => H2 H3.
+    by apply: H1.
+  move => H2 H3.
+  move: (mem_der_Conc _ _ w1 (a::w2) H2 H3).    
+  rewrite -cat_rcons.
+  move/mem_der_Conc2 => [] w3 [] w4 [] .
+  apply: IHw2.
+*)
+
+(*
+Lemma nfa_R_correct2_Star k i j w1 w2:
+  (forall (w : word char) (i j : 'I_#|A|),
+        mem_der (R k i j) w -> nfa_accept (nfa_R k i j) (enum_val i) w) ->
+  mem_der (Star (R k (k1_ord k) (k1_ord k))) (w1 ++ w2) -> exists xs, nfa_lpath (nfa_R k.+1 i j) (enum_val (k1_ord k)) xs (w1 ++ w2) /\ last (enum_val (k1_ord k)) xs = enum_val (k1_ord k).
+Proof.
+  move => H0.
+
+  elim: w1 w2 i j k H0 => [|a w1 IHw1] w2 i j k H0.
+  
+  
+  elim: w i j => [|a w IHw] i j.
+    move => _. by exists [::].
+  simpl.
+  
+  move/mem_der_Conc2 => [] w1 [] w2 [] H1 [].
+  rewrite -H1 in IHw. rewrite -H1.
+  move => H2.
+    assert (mem_der (R k (k1_ord k) (k1_ord k)) (a::w1)) => //.
+  
+  elim: w2 w1 H1 IHw H2 H => [|b w2 IHw2] w1 H1 IHw H2 H.
+    move => _.
+    move/nfa_accept_lpath: (H0 _ _ _ H) => [] xs [].
+    move/(nfa_R_correct2''' _ i j) => H3.
+    move/eqP => H4.
+    rewrite cats0. 
+    by exists xs.
+
+  move => /= /mem_der_Conc2 [] w3 [] w4 [] H3 [].
+    
+Admitted.
+*)
+
+Lemma R_monotone k i j w: mem_der (R k i j) w -> mem_der (R k.+1 i j) w.
+Proof. rewrite /= mem_der_Plus => ->. by rewrite orbT. Qed.
+
+Check seq_ind.
+
+Lemma cat_ind (P: word char -> Prop):
+  P [::] ->
+  (forall w1 w2, P w2 -> P (w1 ++ w2)) ->
+  forall w, P w.
+Proof.
+  move => H0 H1 w.
+  elim: w => [|a w IHw] //.
+  rewrite -cat1s.
+  by apply: H1.
+Qed.
+
+
+Lemma R0_cons i j a w:
+  mem_der (R 0 i j) (a::w) ->
+  w = [::] /\ nfa_step (nfa_R 0 i j) (enum_val i) a (enum_val j).
+Proof.
+  move => /=.
+  rewrite fun_if der_Plus der_fold_Plus -map_comp.
+  rewrite fun_if if_arg mem_der_Plus -mem_der_fold_Plus mem_der_Void orFb.
+  rewrite 2!enum_valK 2!eq_refl /= 2!andbT.
+  case_eq (i == j) => H1; rewrite H1.
+    move/orP => [] //.
+    move/hasP => [] r /mapP [] b. rewrite mem_filter => /andP [] /=.
+    case_eq (a == b).
+      by move/eqP => -> -> _ -> /mem_der_Eps ->.
+    move => _ _ _ ->.
+    by rewrite mem_der_Void.
+  move/hasP => [] r /mapP [] b. rewrite mem_filter => /andP [] /=.
+  case_eq (a == b).
+    by move/eqP => -> -> _ -> /mem_der_Eps ->.
+  move => _ _ _ ->.
+  by rewrite mem_der_Void.
+Qed.  
+  
+Lemma R0_nil i j:
+  mem_der (R 0 i j) [::] =
+  (j == i).
+Proof.
+  rewrite /= fun_if -has_eps_fold_Plus /= orbT.
+  case_eq (i == j) => H0; rewrite H0.
+    by rewrite eq_sym H0.
+  apply/hasP/idP.
+    by move => /= [] r /mapP [] a _ ->.
+  by rewrite eq_sym H0.
+Qed.
+                     
+Lemma R_der_step k i j a w m:
+  mem_der (R k i j) (a::w) ->
+  nfa_step (nfa_R k i j) (enum_val i) a (enum_val m) ->
+  mem_der (R k m j) w.
+Proof.
+  elim: k w i j a m => [|k IHk] w i j a m H0.
+    move: (R0_cons _ _ _ _ H0) => [] H1 H2.
+    rewrite H1. rewrite H1 in H0.
+    move => /andP [] /andP [] H3 /orP [] H4 /orP [] H5 //.
+    rewrite enum_valK in H5.
+    by rewrite R0_nil eq_sym H5.
+  move: H0. rewrite /= mem_der_Plus.
+  move/orP => [].
+    case_eq (has_eps (R k i (k1_ord k))) => H0.
+    rewrite mem_der_Plus => /orP [].
+    move/mem_der_Conc2 => [] w1 [] w2 [] <-.
+    
+    move => /andP [] /andP [] H3 /orP [] H4 /orP [] H5 //.
+           rewrite enum_valk
+           
+    
+      
+
+Lemma R_der k i j a w:
+  mem_der (der a (R k i j)) w ->
+  mem_der (R k j j) w \/ 
+  exists m: 'I_#|A|,
+    m < k /\
+    mem_der (R k i m) [::a] /\
+    mem_der (R k m j) w.
+Proof.
+  elim: k i j a w => [|k IHk] i j a w.
+    move => /=.
+    rewrite eq_refl.
+    rewrite fun_if der_Plus der_fold_Plus.
+    case_eq (i==j) => H0; rewrite H0.
+      move/eqP: H0 => ->.
+      rewrite mem_der_Plus => /orP [].
+        rewrite -mem_der_fold_Plus => /orP [].
+          by rewrite mem_der_Void.
+        move/hasP => [] r /mapP [] s /mapP [] b.
+        rewrite mem_filter => /andP [].
+        move => H0 _ -> -> /=.
+        case_eq (a == b).
+          move => _ /mem_der_Eps -> /=.
+          left. by rewrite orbT.
+        by rewrite mem_der_Void.
+      by rewrite /= mem_der_Void.
+    rewrite -mem_der_fold_Plus.
+    move/orP => [].
+      by rewrite mem_der_Void.
+    move/hasP => [] r /mapP [] s /mapP [] b.
+    rewrite mem_filter => /andP [].
+    move => H1 _ -> -> /=.
+    case_eq (a == b).
+      move => _ /mem_der_Eps -> /=.
+      left. by rewrite orbT.
+    by rewrite mem_der_Void.
+  rewrite /= mem_der_Plus => /orP [].
+    case_eq (has_eps (R k i (k1_ord k))) => H0.
+      rewrite mem_der_Plus => /orP [].
+        right.
+        exists (k1_ord k).
+        split.
+          by apply: k1_ord_leq_k.
+        split.
+          
+      
+      
+
+Lemma nfa_R_correct_Star k w:
+  mem_der (Star (R k (k1_ord k) (k1_ord k))) w ->
+  w = [::] \/ mem_der (R k.+1 (k1_ord k) (k1_ord k)) w.
+Proof.
+  (*move: w k. apply: cat_ind => [|w1 w2 IHw] k.*)
+  elim: w k => [|a w IHw] k.
+  
+    move/mem_der_Star => [].
+      by firstorder.
+    move/mem_der_Conc2 => [] w1 [] w2 [].
+    case: w1 => [] //. case: w2 => [] //.
+    by firstorder.
+  rewrite 1!/= => H0.
+  rewrite mem_der_Plus.
+  right.
+  apply/orP.
+  case_eq (has_eps (R k (k1_ord k) (k1_ord k))) => H1.
+    left.
+    rewrite mem_der_Plus.
+    apply/orP. left.
+    apply: mem_der_Conc3.
+    move/mem_der_Conc2: H0 => [] w1 [] w2 [] <- [] H2 H3.
+    exists w1. exists w2.
+    firstorder.
+    apply: mem_der_Conc3.
+    exists w2. exists [::].
+    firstorder.
+    by rewrite cats0.
+  move/mem_der_Conc2: H0 => [] w1 [] w2 [] H2 [] H3 H4.
+  rewrite -H2.
+  elim: w2 w1 H3 H2 H4 => [|b w2 IHw2] w1 H3 H2 H4.
+    right. by rewrite cats0.
+  move/mem_der_Star: H4 => [] //=.
+  rewrite H1 => /mem_der_Conc2 [] w3 [] w4 [] H4 [] H5 H6.
+  
+  
+  left.
+  apply: mem_der_Conc => //=.
+   
+    
+  
+Lemma nfa_R_correct2 k w i j: mem_der (R k i j) w -> nfa_accept (nfa_R k i j) (enum_val i) w.
+Proof.
+  elim: k w i j => [|k IHk] w i j.
+    exact: nfa_R_correct2_0.
+  simpl.
+  rewrite mem_der_Plus.
+  move/orP => [].
+    move/mem_der_Conc2 => [] w1 [] w2 [] H0 [] /IHk /nfa_accept_lpath [] xs1 [] H1 H2.
+    rewrite -H0. clear H0.
+    move/mem_der_Conc2 => [] w3 [] w4 [] H3 [] H4 /IHk /nfa_accept_lpath [] xs2 [] H5 H6.
+    rewrite -H3. clear H3.
+    apply/nfa_accept_cat.
+    exists xs1.
+    move/eqP: H2 => /= ->.
+    move: H1 => /(nfa_R_correct2' _ _ j) => -> /=.
+    
+    apply/nfa_accept_cat.
+    exists xs2.
+    apply/andP. split.
+      clear H5 H6
+    
+    
+    move: (mem_der_Star _ _ H4) => [].
+      move => H7. rewrite H7.
+      apply: nfa_lpath_accept.
+        eapply nfa_R_correct2''.
+        eassumption.
+      exact: H6.
+    move/mem_der_Conc2 => [] w5 [] w6 [] H7 [] /IHk H8 _.
+
+    apply: mem_der
+        
+        
+      
+    
+    exists xs2.
+      move => ->. case: xs2 H5 H6 => [|x xs2] H5 H6.
+      simpl.
+          
+      
+    
+
+  case: w IHw => [|b w] IHw.
+    rewrite orFb orbF.
+    move/hasP => [] r /mapP [] s /mapP [] c.
+    rewrite mem_filter /= => /andP [] H0.
+    move => _ -> -> /=.
+    case_eq (a==c) => [/eqP ->|] //= _.
+    apply/existsP. exists (enum_val j).
+    by rewrite enum_valK 2!eq_refl H0.
+       
+            
+     
+Lemma nfa_R_correct2 k i j w : mem_der (R k i j) w -> nfa_fin A (enum_val j) -> nfa_accept (nfa_R k i j) (enum_val i) w.
+Proof.
+  elim: k w i j => [|k IHk] w i j.
+    case_eq (i == j).
+      move/eqP => ->.
+      rewrite /= eq_refl.
+      rewrite mem_der_Plus -mem_der_fold_Plus.
+      move/orP => [].
+        move/orP => [].
+        elim: w => [|a w IHw] //=.
+        
+      
+
+Lemma nfa_R_correct k (i j: 'I_#|A|) w: nfa_fin A (enum_val j) -> nfa_accept (nfa_R k i j) (enum_val i) w -> mem_der (R k i j) w.
+Proof.
+
+  elim: k w i j => [|k IHk] w i j.
+    elim: w i j => [|a w IHw] i j.
+      case_eq (i==j).
+        move/eqP => -> H0 _ /=.
+        by rewrite eq_refl /= orbT.
+      move => H1 H0 /eqP /(f_equal enum_rank).
+      rewrite 2!enum_valK => H2. move: H1.
+      by rewrite H2 eq_refl.
+    move => H0 /existsP [] y /andP [] /andP [] /orP [] H1 H2 H3.
+    simpl.
+    case_eq (i==j).
+      move/eqP => H4. rewrite H4 eq_refl der_Plus der_fold_Plus mem_der_Plus.
+      apply/orP. left.
+      rewrite -mem_der_fold_Plus.
+      apply/orP. right.
+      
+      apply: mem_der_fold_Plus.
+      right.
+      rewrite 2!has_map.
+      apply/hasP.
+      exists a.
+      rewrite mem_filter.
+      simpl.
+      
+      
+      
+      
+      
+      by rewrite eq_refl /= orbT.
+      
+  elim: w k i j => [|a w IHw] k i j.
+    elim: k i j => [|k IHk] i j //.
+    simpl.
+    case_eq (i==j).
+      move/eqP => -> H0 _.
+      by rewrite eq_refl /= orbT.
+    move => H1 H0 /eqP /(f_equal enum_rank).
+    rewrite 2!enum_valK => H2. move: H1.
+    by rewrite H2 eq_refl.
+  move => H0 /=.
+  move /eqP /(f_equal enum_rank). rewrite 2!enum_valK => ->.
+  apply/orP. right.
+  apply: IHk.
+    exact: H0.
+  by rewrite /= eq_refl.
+move => H0.
+rewrite /nfa_lang /=.
+move/existsP => [] y /andP [] /andP [] /orP [] H1 H2 H3.
+  apply: IHw.
+  
+  
+  simpl.
+
+  
+
+Lemma R_correct0' x a y : dfa_step A x a = y ->
+   has_eps
+     (der a
+        (foldr (@Plus char) (Void char)
+           (map (Atom (symbol:=char))
+              (filter
+                 [pred a0 : char |
+                  dfa_step A (enum_val (enum_rank x)) a0 ==
+                  enum_val (enum_rank y)] (enum char))))).
+Proof. move => H0.
+  rewrite der_fold_Plus.
+  apply: has_eps_fold_Plus.
+  right. exists (Eps _).
+  rewrite /= andbT.
+  apply/mapP.
+  exists (Atom a).
+    apply/mapP.
+    exists a.
+      by rewrite mem_filter /= 2!enum_rankK H0 eq_refl andTb mem_enum.
+    by [].
+  by rewrite /= eq_refl.
+Qed.
+   
+
+Lemma R_correct0 x a y: dfa_step A x a = y -> has_eps (der a (R 0 (enum_rank x) (enum_rank y))).
+Proof.
+case_eq (x == y) => /=.
+  move/eqP => ->. rewrite eq_refl => /=.
+  rewrite orbF. exact: R_correct0'.
+move => H0.
+assert (enum_rank x == enum_rank y = false).
+  apply/eqP.
+  move/(f_equal enum_val).
+  rewrite 2!enum_rankK.
+  move => H1. move: H1 H0 => ->. by rewrite eq_refl. 
+rewrite H.
+exact: R_correct0'.
+Qed.
+
+Lemma R_correct1 k x a w y:
+  let x' := dfa_step A x a in
+  let xs := dfa_run' A x' w in
+  all [ pred x | enum_rank x < k] (belast x' xs) ->
+  last x' xs = y ->
+  mem_der (R k (enum_rank x) (enum_rank y)) (a::w).
+Proof.
+elim: w k a x y => [|b w IHw] k a x y.
+  elim: k a x y => [|k IHk] a x y x' xs H0 H1.
+    by apply: R_correct0.
+  simpl in H0,H1.
+  rewrite -H1.
+  rewrite /=. apply/orP. right.
+  move: (IHk _ _ _ H0 H1).
+  by rewrite -H1.
+elim: k w IHw a x y => [|k IHk] w IHw a x y x' xs H0 H1 //.
+move: (IHk _ IHw). clear IHk => IHk.
+simpl R.
+rewrite mem_der_Plus.
+
+
+
+assert ([pred x0 | enum_rank x0 < k.+1] =1 [pred x0 : A | (enum_rank x0 < k) || (k == enum_rank x0) ]).
+  move => x0.
+  rewrite /= leq_eqVlt -{2}(addn1 (enum_rank x0)) -{2}(addn1 k) ltn_add2r.
+  rewrite orbC eq_sym.
+  case_eq (enum_rank x0 < k) => -> //=.
+move: H0.
+rewrite (eq_all H).
+rewrite all_predI.
+
+
+move => x' xs H0 H1.
+simpl.
+elim: k w IHw a x y => [|k IHk] a x y x' xs H0 H1.
+   
+
+  
+elim: k x a w y => [|k IHk] x a w y.
+  elim: w a x y => [|b w IHw] a x y //=.
+  move => _.
+  exact: R_correct0.
+elim: w k IHk a x y => [|b w IHw] k IHk a x y.
+  rewrite /dfa_run' /last.
+  rewrite /belast => _.
+  move => H0.
+  apply/orP. right.
+  exact: (IHk x a [::] y is_true_true H0).
+move => x' xs.
+rewrite [last x' xs]/= [all _ _]/=.
+move/andP => [] H0 H1 H2.  
+
+(* alternative 1 *)
+move: (IHw _ IHk). clear IHw => IHw.
+
+move Eqw': (b::w) => w'.
+rewrite /= mem_der_Plus.
+move Eqk': (Ordinal (n:=#|A|) (m:=minn k #|A|.-1)
+                    (noname (minn k #|A|.-1) #|A| A_has_states
+                       (minn_to_ord k #|A|.-1))) => k'.
+
+(* Decide whether the new run goes over the newly
+   included state. *)
+move: H0. rewrite leq_eqVlt orbC -{1}(addn1 k) -{1}(addn1 (enum_rank x')) ltn_add2r => /orP [].
+  move => H0.
+  apply/orP. right.
+  apply: IHk.
+  
+
+case_eq (x' == enum_val k').
+  move/eqP => H3.
+  rewrite 2!fun_if if_arg.
+  case_eq (has_eps (R k (enum_rank x ) k')) => H4.
+    rewrite mem_der_Plus.
+    rewrite -Eqw'. rewrite (mem_der_Conc _ _ [::b] w).
+    rewrite mem_der_Plus.
+    rewrite (mem_der_Conc _ _ [::b] w).
+    
+    apply/orP. left.
+    rewrite [der b _]/= .
+    
+    assert (has_eps (der a (R k (enum_rank x) k'))).
+      move: (IHk x a [::] (enum_val k') is_true_true H3).
+      by rewrite /= enum_valK.
+    rewrite H 2!mem_der_Plus.
+    apply/orP. left. apply/orP. left.
+    eapply (mem_der_Conc _ _).
+    
+    
+
+
+
+
+
+(* alternative 2 *)
+
+move: H0. rewrite leq_eqVlt => /orP [].
+  move/eqP/(f_equal predn) => H0. simpl in H0. 
+  rewrite /= mem_der_Plus. apply/orP. left.
+  move Eqk': (Ordinal (n:=#|A|) (m:=minn k #|A|.-1)
+                    (noname (minn k #|A|.-1) #|A| A_has_states
+                       (minn_to_ord k #|A|.-1))) => k'.
+  rewrite 2!fun_if if_arg der_Plus mem_der_Plus.
+  case_eq (has_eps (R k (enum_rank x ) k')) => H3.
+    rewrite der_Plus.
+    apply/orP. left.
+    rewrite [der b _]/= .
+
+    assert (x' = enum_val k').
+      rewrite -H0.
+    
+    assert (has_eps (der a (R k (enum_rank x) k'))).
+    move: (IHk x' a [::] (enum_val k') is_true_true).
+    
+        
+
+  
+
+
+End TransitiveClosure.
+
+
 
 Section StateRemoval.
   
@@ -13,161 +863,107 @@ Record re_nfa : Type :=
     re_nfa_state :> finType;
     re_nfa_s0: re_nfa_state;
     re_nfa_fin: pred re_nfa_state;
-    re_nfa_step: re_nfa_state -> word -> pred re_nfa_state
+    re_nfa_re: re_nfa_state -> re_nfa_state -> regular_expression char
     }.
 
 Variable A: nfa char.
 
-Definition nfa_to_re_nfa: 
+Definition nfa_to_re_nfa: re_nfa :=
+  re_nfaI
+    (option_finType A)
+    (Some (nfa_s0 A))
+    (fun x => if x is Some x then false else true)
+    (fun x y =>
+       if x is Some x then
+         if y is Some y then
+            foldr
+              (@Plus char)
+              (@Void char)
+              (map (@Atom char) (enum [pred a | nfa_step A x a y]))
+         else
+           if nfa_fin A x then
+             (@Eps char)
+           else
+             @Void char
+       else
+         if y is Some y then
+           @Void char
+         else
+           @Eps char
+    )
+    .
+    
+Section Acceptance.
+Variable R: re_nfa.
 
-  
-End StateRemoval.
 
-Section TransitiveClosure.
+Definition re_nfa_step: R -> word -> pred R :=
+fun x w y => mem_der (re_nfa_re R x y) w.
 
-Variable char: finType.
-Variable A: dfa char.
-
-Lemma ord_sub (k: 'I_#|A|): k.-1 < #|A|.
+Lemma size_ind (P: word -> Type):
+  (forall w, (forall w', size w' < size w -> P w') -> P w) ->
+  forall w, P w.
 Proof.
-move: (leq_pred k) (ltn_ord k). by apply: leq_ltn_trans.
-Defined.
-
-Lemma R (k: 'I_(#|A|.+1)) (i j: 'I_#|A|) : regular_expression char.
-Proof.
-elim: k => [n H].
-elim: n i j H => [|n R] i j H.
-  case_eq ([pick r | dfa_step A (enum_val i) r == enum_val j ]).
-    move => r _.
-    case_eq (i==j) => H1.
-      exact: Plus (Atom r) (Eps _). 
-    exact: Atom r.
-  move => _. exact: Void _.
-move: (Ordinal H) => k.
-assert (n < #|A|).
-  move: H. by rewrite -{1}(addn1 n) -(addn1 #|A|) ltn_add2r.
-move: (Ordinal H0) => k'. 
-exact (Plus (
-                  Conc
-                    (R i k' (ltnW H0))
-                    (
-                      Conc
-                        (Star (R (Ordinal H0) (Ordinal H0) (ltnW H0)))
-                        (R (Ordinal H0) j (ltnW H0))
-                    )
-                )
-                (R i j (ltnW H0))).
-Defined.
-
-Lemma mem_der_Void w: mem_der (Void char) w = false.
-Proof. elim: w => [|a w IHw] //. Qed.
-
-Lemma mem_der_Eps w: mem_der (Eps char) w -> w = [::].
-Proof. elim: w => [|a w IHw] //=. by rewrite mem_der_Void. Qed.
-
-Lemma mem_der_Plus (r1 r2: regular_expression char) w: mem_der (Plus r1 r2) w = mem_der r1 w || mem_der r2 w.
-Proof. elim: w r1 r2 => [|a w IHw] r1 r2 //=. Qed.
-
-Lemma mem_der_Atom (a: char) w: mem_der (Atom a) w -> w = [::a].
-Proof. elim: w a => [|b w IHw] a //=.
-case_eq (b == a).
-  by move/eqP => -> /mem_der_Eps ->.
-by rewrite mem_der_Void.                     
+move => H w.
+move Heqn: (size w) => n.
+assert (size w <= n). by rewrite Heqn.
+clear Heqn.
+elim: n w H0 => [|n IHn] w.
+  rewrite leqn0. move/eqP/size0nil => ->. by apply: H.
+rewrite leq_eqVlt.
+case_eq (size w == n.+1); case_eq (size w < n.+1) => //.
+    move => H1 _ _. by apply: IHn.
+  move => _ /eqP H1 _. apply: H.
+  rewrite H1. exact: IHn.
+move => H1 _ _. by apply: IHn.
 Qed.
 
-Lemma R_rec (k: 'I_#|A|.+1) i j (H0: k.+1 < #|A|.+1) (H1: k < #|A|):
-  let k' := (Ordinal (n:=#|A|.+1) (m:=k.+1) (H0)) in
-  let k'' := (Ordinal (n:=#|A|) (m:=k) (H1)) in
-  (R k' i j) =
-      (Plus (
-                  Conc
-                    (R k i k'')
-                    (
-                      Conc
-                        (Star (R k k'' k''))
-                        (R k k'' j )
-                    )
-                )
-                (R k i j)).
-Proof. elim: k i j H0 H1 => [n H2] i j H0 H1.
-elim: n i j H2 H0 H1 => [|n IHn] i j H2 H0 H1.
-simpl.
-assert (H: forall X Y (f: X -> X -> Y) a b x y, a = b -> x = y -> f a x = f b y).
-  by move => X Y f x y a b -> ->.
+Lemma sub0 n: n - 0 = n.
+elim: n => [|n IHn] //.
+Qed.                    
 
-eapply H.
-  eapply H.
-  
-  case: (pickP [pred a | (dfa_step A (enum_val i) a == enum_val j)]).
-
-  
-Lemma R_correct2 (k: 'I_#|A|.+1) (i j: 'I_#|A|) a w:
-  mem_der (R k i j) (a::w)
-  -> (
-    let x := dfa_step A (enum_val i) a in
-    let xs := dfa_run' A x w in
-    all (fun y => enum_rank y < k)
-        (belast x xs)
-    &&  (enum_rank (last x xs) == j)
-  ).
+Lemma drop_size_gt0 n (w: word) : size w > 0 -> n > 0 -> size (drop n w) < size w.
 Proof.
-elim: k i j w => [k H0] i j w.
-elim: k H0 i j w => [|k IHk] H0 i j w.
-  simpl.
-  case: (pickP [pred a | (dfa_step A (enum_val i) a == enum_val j)]).
-    move => r /= /eqP.
-    case_eq (i == j).
-      move/eqP => ->. rewrite eq_refl.
-      simpl.
-      case_eq (a == r).
-        move/eqP => -> H1.
-        rewrite mem_der_Plus => /orP [].
-          move/mem_der_Eps => -> /=.
-          move/(f_equal enum_rank): H1.
-          by rewrite enum_valK => /eqP.
-        by rewrite mem_der_Void.
-      move => H1 H2.
-      rewrite mem_der_Plus => /orP [];
-      by rewrite mem_der_Void.
-    move => -> /=.
-    case_eq (a == r).
-      move/eqP => -> H1.
-      move/mem_der_Eps => -> /=.
-      move/(f_equal enum_rank): H1.
-      by rewrite enum_valK => /eqP.
-    by rewrite mem_der_Void.
-  move => H1.
-  by rewrite mem_der_Void.
-rewrite /R /ordinal_rect /nat_rect.
+rewrite size_drop.
+move => H.
+rewrite leq_eqVlt => /orP [].
+  move/eqP => H1. move: H. rewrite -H1 subn1 => H.
+  rewrite -(ltn_add2r 1) addn1 prednK -addn1 //.
+move => H1.
+assert (size w -n < size w - 0).
+  apply: ltn_sub2l => //.
+  move: H1.
+  by apply: ltn_trans.
+move: H0.
+by rewrite sub0.
+Qed.
 
+  
+Lemma re_nfa_accept (x: R) (w: word): bool.
+Proof.
+move: w x. apply: size_ind.
+move => [|a w] F x.
+  exact: re_nfa_fin x.
+exact
+(
+  existsb n: 'I_(size (a::w)),
+    existsb y: R,
+      re_nfa_step x (take n.+1 (a::w)) y
+    && F (drop n.+1 (a::w)) (drop_size_gt0 _ (a::w) (ltn0Sn _) (ltn0Sn _)) y
+).
+Defined.
+
+End Acceptance.
+
+Lemma nfa_to_re_nfa_correct1 x w: nfa_accept A x w -> re_nfa_accept (nfa_to_re_nfa) (Some x ) w.
+Proof. 
+elim: w x => [|a w IHw] x /=.
+  move => H0.
+  rewrite /re_nfa_accept /size_ind /=.
 
     
-       
-Lemma R_correct1 (k: 'I_#|A|.+1) (i j: 'I_#|A|) a w:
-  let x := dfa_step A (enum_val i) a in
-  let xs := dfa_run' A x w in
-  all
-    (fun y => enum_rank y < k)
-    (belast x xs)
-  -> enum_rank (last x xs) == j
-  -> mem_der (R k i j) (a::w).
-Proof.
-elim: k i j w => [k H0] i j w.
-elim: k H0 i j w => [|k IHk] H0 i j w.
-  simpl.
-  case: (pickP [pred a | (dfa_step A (enum_val i) a == enum_val j)]).
-    move => r /= /eqP H1. 
-    move: H1. case_eq (i == j) => H2.
-      rewrite (eqP H2).
-      elim: w i j H2 => [|b w IHw] i j H2 //.
-        rewrite eq_refl /=.
-        rewrite -{4}(enum_valK j) => H1 _.
-        rewrite -{2}H1. move/eqP.
-        move/(f_equal enum_val).
-        rewrite 2!enum_rankK.
-                  
-    elim: w i j H2 => [|b w IHw] i j H2 //=.
-      
+                                          
+End StateRemoval.
 
-                        
-End TransitiveClosure.
+
+
